new/proof/github_com/sanjit_bhat/pav/merkle.v
@@ -5,4 +5,12 @@ From New.proof.github_com.sanjit_bhat.pav.merkle_proof Require Import base serde
 
 Module merkle.
   Export base serde theory.
+  (* tentative strategy:
+  - inside sub-files, don't mark opaque / local.
+  those objects need to be visible inside the "pkg".
+  - at export time, only export external objects.
+  - ideally, mark external objects as opaque.
+  if haven't proved all helper lemmas for external obj,
+  then might need to leave as transp and mark lower-level obj as opaque. *)
+  #[global] Opaque is_full_tree is_merkle_map is_merkle_entry.
 End merkle.
