new/proof/github_com/sanjit_bhat/pav/merkle_proof/merkle.v
@@ -1,0 +1,39 @@
+From New.proof.github_com.sanjit_bhat.pav Require Import prelude.
+From New.generatedproof.github_com.sanjit_bhat.pav Require Import merkle.
+From Perennial.Helpers Require Import bytes NamedProps.
+
+From New.proof.github_com.goose_lang Require Import primitive std.
+From New.proof.github_com.sanjit_bhat.pav Require Import cryptoffi cryptoutil safemarshal.
+From New.proof.github_com.tchajed Require Import marshal.
+
+From New.proof.github_com.sanjit_bhat.pav.merkle_proof Require Import base serde theory.
+
+Section proof.
+Context `{hG: heapGS Σ, !ffi_semantics _ _, !goGlobalsGS Σ}.
+Context `{!merkle.GlobalAddrs}.
+
+Definition wish_merkle_Verify (in_tree : bool) label val proof dig : iProp Σ :=
+  ∃ found proof_obj proof' tail,
+  "%Henc" ∷ ⌜ MerkleProof.encodes proof_obj proof' ⌝ ∗
+  "%Heq_tail" ∷ ⌜ proof = proof' ++ tail ⌝ ∗
+  "%Heq_found" ∷
+    ⌜if in_tree
+    then found = Some (label, val)
+    else if proof_obj.(MerkleProof.IsOtherLeaf)
+      then found = Some (proof_obj.(MerkleProof.LeafLabel), proof_obj.(MerkleProof.LeafVal)) ∧
+        label ≠ proof_obj.(MerkleProof.LeafLabel)
+      else found = None ⌝ ∗
+  "#His_proof" ∷ is_merkle_proof label found proof_obj.(MerkleProof.Siblings) dig.
+Global Opaque wish_merkle_Verify.
+Local Transparent wish_merkle_Verify.
+Global Instance wish_merkle_Verify_pers i l v p d : Persistent (wish_merkle_Verify i l v p d) := _.
+
+Lemma wish_merkle_Verify_to_entry in_tree label val proof dig :
+  wish_merkle_Verify in_tree label val proof dig -∗
+  is_merkle_entry label (if in_tree then Some val else None) dig.
+Proof.
+  iNamed 1. iNamed "His_proof".
+  repeat case_match; intuition; subst; by iFrame "#%".
+Qed.
+
+End proof.
